Constr/CSetTac.v
@@ -240,6 +240,15 @@ Hint Extern 10 => match goal with
                    | [ H : ?x ∈ ?s, H' : ?y ∈ ?s -> False, H'' : ?x === ?y |- _ ] => exfalso; eapply H'; rewrite <- H''; eapply H
                  end.
 
+Hint Extern 20 (incl ?a ?a') => (is_evar a ; fail 1) || (has_evar a ; fail 1) ||
+                               (is_evar a' ; fail 1) || (has_evar a'; fail 1) || reflexivity.
+Hint Extern 20 (Subset ?a ?a') => (is_evar a ; fail 1) || (has_evar a ; fail 1) ||
+                                 (is_evar a' ; fail 1) || (has_evar a'; fail 1) || reflexivity.
+
+Hint Extern 20 (Equal ?a ?a') => (is_evar a ; fail 1) || (has_evar a ; fail 1) ||
+                                 (is_evar a' ; fail 1) || (has_evar a'; fail 1) || reflexivity.
+
+
 (*
 *** Local Variables: ***
 *** coq-load-path: (("../" "Lvc")) ***
