EAE.v
@@ -110,20 +110,6 @@ Proof.
       eauto.
 Qed.
 
-
-(*TODO: generalize this, it might be useful *)
-Instance list_get_computable X (Y:list X) (R:X->Prop) `{forall (x:X), Computable (R x)}
-: Computable (forall n y, get Y n y -> R y).
-Proof.
-  hnf. general induction Y.
-  - left; isabsurd.
-  - decide (R a).
-    + edestruct IHY; eauto.
-      * left; intros. inv H0; eauto using get.
-      * right; intros; eauto using get.
-    + right; eauto using get.
-Defined.
-
 Fixpoint compile s
   : stmt :=
   match s with
