Infra/Drop.v
@@ -12,7 +12,7 @@ Fixpoint drop {X} (n : nat) (xs : list X) : list X :=
 Fixpoint drop_error {X} (n : nat) (xs : list X) : option (list X) :=
   match n with
     | 0   => Some xs
-    | S n => match xs with 
+    | S n => match xs with
                | nil => None
                | _::xs => drop_error n xs
              end
@@ -23,13 +23,13 @@ Lemma drop_get X (L:list X) k n v
   : get L (k+n) v -> get (drop k L) n v.
 Proof.
   revert L. induction k; simpl; intros. trivial.
-  inv H. eauto. 
+  inv H. eauto.
 Qed.
 
-Lemma get_drop_eq X (L L':list X) n x y 
+Lemma get_drop_eq X (L L':list X) n x y
   : get L n x -> y::L' = drop n L -> x = y.
 Proof.
-  intros. revert L' y H0. 
+  intros. revert L' y H0.
   induction H; intros; inv H0; eauto.
 Qed.
 
@@ -48,7 +48,7 @@ Proof.
   constructor. eauto.
 Qed.
 
-Lemma length_drop_cons X (L:list X) k a x 
+Lemma length_drop_cons X (L:list X) k a x
   : k <= length L -> length (drop k L) = a -> length (drop k (x::L)) = S a.
 Proof.
   revert x L. induction k. simpl. intros. f_equal; eauto.
@@ -66,7 +66,7 @@ Proof.
 Qed.
 
 Lemma drop_nil X k
-  : drop k nil = (@nil X). 
+  : drop k nil = (@nil X).
 Proof.
   induction k; eauto.
 Qed.
@@ -89,12 +89,12 @@ Lemma drop_tl X (L:list X) n
   : tl (drop n L) = drop n (tl L).
 Proof.
   revert L. induction n; intros; simpl; eauto.
-Qed.  
+Qed.
 
 Lemma drop_drop X (L:list X) n n'
   : drop n (drop n' L) = drop (n+n') L.
 Proof.
-  revert L. induction n; simpl; intros; eauto. 
+  revert L. induction n; simpl; intros; eauto.
   rewrite <- IHn. rewrite drop_tl; eauto.
 Qed.
 
@@ -111,15 +111,15 @@ Qed.
 Lemma drop_swap X m n (L:list X)
   : drop m (drop n L) = drop n (drop m L).
 Proof.
-  revert n L; induction m; intros; simpl; eauto. 
+  revert n L; induction m; intros; simpl; eauto.
   rewrite drop_tl. eauto.
-Qed.  
+Qed.
 
 
 Lemma drop_nth X k L (x:X) L' d
   : drop k L = x::L' -> nth k L d = x.
 Proof.
-  revert x L L'; induction k; intros; simpl in * |- *; subst; eauto. 
+  revert x L L'; induction k; intros; simpl in * |- *; subst; eauto.
   destruct L. simpl in H. rewrite drop_nil in H. inv H.
   simpl in *. eauto.
 Qed.
@@ -132,7 +132,7 @@ Proof.
   rewrite IHn; f_equal; eauto using tl_map.
 Qed.
 
-Lemma drop_length_eq X (L L' :list X) 
+Lemma drop_length_eq X (L L' :list X)
 : drop (length L') (L' ++ L) = L.
 Proof.
   general induction L'; simpl; eauto.
@@ -154,7 +154,43 @@ Proof.
   simpl. eapply IHL'. simpl in *; omega.
 Qed.
 
-(* 
+Lemma drop_eq X (L L':list X) n y
+: y::L' = drop n L -> get L n y.
+Proof.
+  intros. general induction n; simpl in *.
+  + inv H; eauto using get.
+  + destruct L.
+  - simpl in H. rewrite drop_nil in H. inv H.
+  - econstructor; eauto.
+Qed.
+
+Lemma drop_shift_1 X (L:list X) y YL i
+: y :: YL = drop i L
+  -> YL = drop (S i) L.
+Proof.
+  general induction i; simpl in *.
+  - inv H; eauto.
+  - destruct L; simpl in *; eauto.
+    + rewrite drop_nil in H; inv H.
+Qed.
+
+Lemma drop_length_stable X Y (L:list X) (L':list Y) i
+: length L = length L'
+  -> length (drop i L) = length (drop i L').
+Proof.
+  general induction i; simpl; eauto. erewrite IHi; eauto.
+  destruct L,L'; try inv H; eauto.
+Qed.
+
+
+Lemma get_eq_drop X (L :list X) n x
+: get L n x -> x::drop (S n) L = drop n L.
+Proof.
+  intros. general induction H; simpl; eauto.
+Qed.
+
+
+(*
 *** Local Variables: ***
 *** coq-load-path: (("../" "Lvc")) ***
 *** End: ***
