Infra/Indexwise.v
@@ -1,0 +1,39 @@
+Require Import Arith Coq.Lists.List Setoid Coq.Lists.SetoidList Omega Containers.OrderedTypeEx.
+Require Export Infra.Option EqDec AutoIndTac Get.
+
+Set Implicit Arguments.
+
+Definition indexwise_R {A} {B} (R:A->B->Prop) LA LB :=
+forall n a b, get LA n a -> get LB n b -> R a b.
+
+Definition indexwise_R_dec {A} {B} {R:A->B->Prop} (Rdec:(forall a b, Computable (R a b))) LA LB
+      : Computable (indexwise_R R LA LB) .
+unfold Computable. revert LA LB. fix 2. intros LA LB.
+destruct LA, LB; try now left; isabsurd.
+intros. destruct (Rdec a b).
+- destruct (indexwise_R_dec LA LB).
+  + left. hnf; intros. destruct n; inv H; inv H0; eauto.
+  + right; intro HH. eapply n; hnf; intros; eapply HH; eauto using get.
+- right; intro. eapply n; hnf; intros. eapply H; eauto using get.
+Defined.
+
+Definition indexwise_R_dec' {A} {B} {R:A->B->Prop} LA LB (Rdec:(forall n a b, get LA n a -> get LB n b -> Computable (R a b)))
+      : Computable (indexwise_R R LA LB).
+unfold Computable. revert LA LB Rdec. fix 2. intros LA LB Rdec.
+destruct LA, LB; try now left; isabsurd.
+intros. destruct (Rdec 0 a b).
+- eauto using get.
+- eauto using get.
+- destruct (indexwise_R_dec' LA LB).
+  + intros. eauto using get.
+  + left. hnf; intros. destruct n; inv H; inv H0; eauto.
+  + right; intro HH. eapply n; hnf; intros; eapply HH; eauto using get.
+- right; intro. eapply n; hnf; intros. eapply H; eauto using get.
+Defined.
+
+
+(*
+*** Local Variables: ***
+*** coq-load-path: (("../" "Lvc")) ***
+*** End: ***
+*)
